wip fresh name gen,
std lib support for decimal strings seems poor

compiler/src/compiler/StringNameGen.v
@@ -1,16 +1,96 @@
+Require Import Coq.Strings.Ascii.
+Require Import Coq.Strings.String.
 Require Import Coq.Lists.List.
 Require Import compiler.util.Common.
 Require Import compiler.NameGen.
+Require Import Coq.NArith.NArith.
+Require Import Coq.Numbers.DecimalString.
+Require Import Coq.Numbers.DecimalN.
 
 Local Open Scope string_scope.
+Local Open Scope char_scope.
+Local Open Scope N_scope.
 
 Local Axiom TODO_someone_freshnames: False.
 
-Instance StringNameGen: NameGen string string. refine ({|
-  freshNameGenState := fun l => "_x"; (* TODO this might clash with names in l *)
-  genFresh s := (s, append s "'");
-  allFreshVars s := fun x => (String.length s <= String.length x)
+Definition maxLength: list string -> nat :=
+  List.fold_right (fun s res => max res (String.length s)) 0%nat.
+
+Definition N_to_string(n: N): string := DecimalString.NilEmpty.string_of_uint (N.to_uint n).
+
+Lemma string_of_uint_inj: forall ui1 ui2,
+    NilEmpty.string_of_uint ui1 = NilEmpty.string_of_uint ui2 -> ui1 = ui2.
+Proof.
+  intros.
+  apply Option.eq_of_eq_Some.
+  rewrite <- (NilEmpty.usu ui1), <- (NilEmpty.usu ui2).
+  f_equal.
+  assumption.
+Qed.
+
+Lemma N_to_string_inj: forall n1 n2, N_to_string n1 = N_to_string n2 -> n1 = n2.
+Proof.
+  unfold N_to_string.
+  intros.
+  apply Unsigned.to_uint_inj.
+  apply string_of_uint_inj.
+  assumption.
+Qed.
+
+Lemma N_to_uint_nb_digits: forall e n,
+    10 ^ N.of_nat e <= n < 10 * 10 ^ N.of_nat e ->
+    Decimal.nb_digits (N.to_uint n) = S e.
+Proof.
+  intros.
+  unfold N.to_uint.
+  destruct n.
+  - apply proj1 in H.
+    pose proof (N.pow_nonzero 10 (N.of_nat e)).
+    blia.
+  - unfold Pos.to_uint.
+    replace (Decimal.nb_digits (Decimal.rev (Pos.to_little_uint p))) with
+        (Decimal.nb_digits (Pos.to_little_uint p)) by admit.
+    revert dependent p.
+    induction e; intros.
+    + simpl in *.
+Abort.
+
+Lemma ten_to_number_of_digits_lower_bound: forall n,
+    n < 10 ^ N.of_nat (String.length (N_to_string n)).
+Proof.
+  unfold N_to_string. intros.
+Admitted.
+
+Instance StringNameGen: NameGen string N. refine ({|
+  freshNameGenState(l: list string) := (10 ^ (N.of_nat (maxLength l)))%N;
+  genFresh(state: N) := (String "x" (N_to_string state), state + 1);
+  allFreshVars(state: N) := fun v => exists state', String "x" (N_to_string state') = v /\ state <= state';
 |}).
-- case TODO_someone_freshnames.
-- case TODO_someone_freshnames.
+(* TODO abstract proofs *)
+all: unfold PropSet.subset, PropSet.elem_of; intros.
+- inversion H; subst; clear H. ssplit.
+  + eexists. split; reflexivity.
+  + intro C. destruct C as [s' [E H]].
+    inversion E. clear E.
+    apply N_to_string_inj in H1. blia.
+  + intros. destruct H as [s' [E H]]. subst x.
+    eexists. split; [reflexivity|]. blia.
+- intro C. destruct C as [state [E C]]. subst v.
+  revert dependent l. induction l; simpl; intros.
+  + assumption.
+  + destruct H.
+    * subst. simpl in *.
+      assert (10 ^ (N.of_nat (S (String.length (N_to_string state)))) <= state) as A. {
+        eapply N.le_trans. 2: eassumption.
+        apply N.pow_le_mono_r; blia.
+      }
+      replace (N.of_nat (S (String.length (N_to_string state)))) with
+          (1 + N.of_nat (String.length (N_to_string state))) in A by blia.
+      rewrite N.pow_add_r in A.
+      change (10 ^ 1) with 10 in A.
+      pose proof (ten_to_number_of_digits_lower_bound state).
+      blia.
+    * eapply IHl. 1: eassumption.
+      eapply N.le_trans. 2: eassumption.
+      apply N.pow_le_mono_r; blia.
 Defined.
